hol/actiongraphs/actionScript.sml
@@ -1,0 +1,79 @@
+open HolKernel Parse boolLib bossLib;
+
+open pred_setTheory listRangeTheory listTheory
+open finite_mapTheory
+open lcsymtacs
+open indexedListsTheory
+
+val _ = new_theory "action";
+
+val _ = Hol_datatype`
+  action = <|
+    writes : 'rw list;
+    reads : 'rw list ;
+    data : 'data;
+    ident : 's_ident
+     (* bogus ty variable name chosen to preserve order of
+        type arguments *)
+  |>
+`;
+
+val action_component_equality = theorem "action_component_equality"
+
+val touches_def = Define`
+  touches a1 a2 ⇔
+     (∃w. MEM w a1.writes ∧ MEM w a2.writes) ∨
+     (∃w. MEM w a1.writes ∧ MEM w a2.reads) ∨
+     (∃w. MEM w a2.writes ∧ MEM w a1.reads)
+`;
+
+val _ = set_mapped_fixity {term_name = "touches", fixity = Infix(NONASSOC, 450),
+                           tok = "∼ₜ"}
+val _ = set_mapped_fixity {term_name = "not_touches",
+                           fixity = Infix(NONASSOC, 450),
+                           tok = "≁ₜ"}
+val _ = overload_on("not_touches", ``λa1 a2. ¬(touches a1 a2)``)
+
+val touches_ignores_ident = store_thm(
+  "touches_ignores_ident",
+  ``(touches a1 (a2 with ident updated_by f) ⇔ touches a1 a2) ∧
+    (touches (a1 with ident updated_by f) a2 ⇔ touches a1 a2)``,
+  simp[touches_def]);
+val _ = export_rewrites ["touches_ignores_ident"]
+
+val touches_SYM = store_thm(
+  "touches_SYM",
+  ``touches a1 a2 ⇒ touches a2 a1``,
+  simp[touches_def] >> rpt strip_tac >> simp[] >> metis_tac[]);
+
+(* redundant if HOL's github issue #173 is fixed *)
+val polydata_upd_def = Define`
+  polydata_upd f a = <|
+    reads := a.reads ;
+    writes := a.writes ;
+    data := f a.data;
+    ident := a.ident
+  |>`
+
+val polydata_upd_ident = store_thm(
+  "polydata_upd_ident[simp]",
+  ``(polydata_upd f a).ident = a.ident``,
+  simp[polydata_upd_def]);
+
+val polydata_upd_reads_writes = store_thm(
+  "polydata_upd_reads_writes[simp]",
+  ``(polydata_upd f a).reads = a.reads ∧ (polydata_upd f a).writes = a.writes``,
+  simp[polydata_upd_def]);
+
+val polydata_upd_data = store_thm(
+  "polydata_upd_data[simp]",
+  ``(polydata_upd f a).data = f a.data``,
+  simp[polydata_upd_def]);
+
+val touches_dataupd = store_thm(
+  "touches_dataupd[simp]",
+  ``(polydata_upd f a ∼ₜ b ⇔ a ∼ₜ b) ∧
+    (b ∼ₜ polydata_upd f a ⇔ b ∼ₜ a)``,
+  simp[touches_def]);
+
+val _ = export_theory();
